more incremental

Weidenbach_Book/CDCL_WNOT.thy
@@ -3867,11 +3867,19 @@ next
   then show ?case by simp force
 qed
 
-text \<open>We can fully run @{term cdcl_fw_s} or add a clause.\<close>
+text \<open>We can fully run @{term cdcl_s} or add a clause. Remark that we use @{term cdcl_s} to avoid 
+an explicit @{term skip}, @{term resolve}, and @{term backtrack} normalisation. to get rid of the
+conflict @{term S} if necessary.\<close>
 inductive incremental_cdcl :: "'st \<Rightarrow> 'st \<Rightarrow> bool" for S where
-"full1 cdcl_fw_s S T \<Longrightarrow> incremental_cdcl S T" |
-"trail S \<Turnstile>asm init_clss S \<Longrightarrow> distinct_mset C \<Longrightarrow> conflicting S = C_True
-  \<Longrightarrow> incremental_cdcl S (add_new_clause_and_update C S)"
+add_confl:
+  "trail S \<Turnstile>asm init_clss S \<Longrightarrow> distinct_mset C \<Longrightarrow> conflicting S = C_True \<Longrightarrow>
+    trail S \<Turnstile>as CNot C \<Longrightarrow> 
+    full cdcl_s 
+      (update_conflicting (C_Clause C) (add_init_cls C (cut_trail_wrt_clause C (trail S) S))) T \<Longrightarrow> 
+    incremental_cdcl S T" |
+add_no_confl:
+  "trail S \<Turnstile>asm init_clss S \<Longrightarrow> distinct_mset C \<Longrightarrow> conflicting S = C_True \<Longrightarrow> \<not>trail S \<Turnstile>as CNot C
+    \<Longrightarrow> incremental_cdcl S (add_init_cls C S)"
 
 inductive add_learned_clss :: "'st \<Rightarrow> 'v clauses \<Rightarrow> 'st \<Rightarrow> bool" for S :: 'st where
 add_learned_clss_nil: "add_learned_clss S {#} S" |
@@ -4012,7 +4020,6 @@ proof -
     unfolding cdcl_all_struct_inv_def by (auto simp: add_new_clause_and_update_def)
 qed
 
-(* distinguish between C = {#} and C \<noteq> {#} *)
 lemma cdcl_all_struct_inv_add_new_clause_and_update_cdcl_s_inv:
   assumes
     inv_s: "cdcl_s_invariant T" and
@@ -4045,7 +4052,7 @@ proof -
     next
       case not_false note C = this(1) and l = this(2)
       let ?L = "- lit_of (hd (trail (cut_trail_wrt_clause C (trail T) T)))"
-      have "get_level ?L (trail (cut_trail_wrt_clause C (trail T) T))
+      have L: "get_level ?L (trail (cut_trail_wrt_clause C (trail T) T))
         = backtrack_lvl (cut_trail_wrt_clause C (trail T) T)"
         using l apply (cases "trail (cut_trail_wrt_clause C (trail T) T)")
         apply auto
@@ -4089,14 +4096,40 @@ proof -
               by (metis IntI Marked_Propagated_in_iff_in_lits_of defined_lit_map empty_iff)
         qed
       qed
-      show ?thesis
+      show ?thesis using L C 
         unfolding cdcl_s_invariant_def
-        unfolding cdcl_all_struct_inv_def apply (auto simp: add_new_clause_and_update_def)
-       sorry
+        unfolding cdcl_all_struct_inv_def by (auto simp: add_new_clause_and_update_def)
     qed
 qed
 
-lemma
+lemma full_cdcl_s_inv_normal_form:
+  assumes
+    full: "full cdcl_s S T" and
+    inv_s: "cdcl_s_invariant S" and
+    inv: "cdcl_all_struct_inv S"
+  shows "conflicting T = C_Clause {#} \<and> unsatisfiable (set_mset (init_clss S)) 
+    \<or> conflicting T = C_True \<and> trail T \<Turnstile>asm init_clss S \<and> satisfiable (set_mset (init_clss S))"
+proof -
+  have "no_step cdcl_s T" 
+    using full unfolding full_def by blast
+  moreover have "cdcl_all_struct_inv T" and inv_s: "cdcl_s_invariant T"
+    apply (metis cdcl_cw_ops.rtranclp_cdcl_s_rtranclp_cdcl cdcl_cw_ops_axioms full full_def inv 
+      rtranclp_cdcl_all_struct_inv_inv)
+    by (metis full full_def inv inv_s rtranclp_cdcl_s_cdcl_s_invariant)
+  ultimately have "conflicting T = C_Clause {#} \<and> unsatisfiable (set_mset (init_clss T)) 
+    \<or> conflicting T = C_True \<and> trail T \<Turnstile>asm init_clss T"
+    using cdcl_s_normal_forms[of T] full unfolding cdcl_all_struct_inv_def cdcl_s_invariant_def full_def
+    by fast
+  moreover have "consistent_interp (lits_of (trail T))"
+    using \<open>cdcl_all_struct_inv T\<close> unfolding cdcl_all_struct_inv_def cdcl_M_level_inv_def
+    by auto
+  moreover have "init_clss S = init_clss T"
+    by (metis rtranclp_cdcl_s_no_more_init_clss full full_def)
+  ultimately show ?thesis
+    by (metis satisfiable_carac' true_annot_def true_annots_def true_clss_def)
+qed    
+  
+lemma incremental_cdcl_inv:
   assumes
     inc: "incremental_cdcl S T" and
     inv: "cdcl_all_struct_inv S" and
@@ -4104,19 +4137,29 @@ lemma
   shows
     "cdcl_all_struct_inv T" and
     "cdcl_s_invariant T"
-  using inc apply (induction)
-      using tranclp_into_rtranclp inv s_inv rtranclp_cdcl_fw_s_cdcl_all_struct_inv
-      unfolding full1_def apply (fast dest: tranclp_into_rtranclp)
-     using tranclp_into_rtranclp inv s_inv rtranclp_cdcl_fw_s_cdcl_s_invariant
-     unfolding full1_def apply (fast dest: tranclp_into_rtranclp)
-    apply (auto simp: add_new_clause_and_update_def)
-      using add_new_clause_and_update_def
-      cdcl_all_struct_inv_add_new_clause_and_update_cdcl_all_struct_inv inv apply auto[1]
-     defer
-     using add_new_clause_and_update_def
-     cdcl_all_struct_inv_add_new_clause_and_update_cdcl_s_inv inv s_inv apply auto[1]
-    unfolding cdcl_s_invariant_def apply (auto split: split_if_asm)
-oops
+  using inc 
+proof (induction)
+  case (add_confl C T)
+  let ?T = "(update_conflicting (C_Clause C) (add_init_cls C (cut_trail_wrt_clause C (trail S) S)))"
+  have "cdcl_all_struct_inv ?T" and inv_s_T: "cdcl_s_invariant ?T"
+    using add_confl.hyps(1,2,4) add_new_clause_and_update_def 
+    cdcl_all_struct_inv_add_new_clause_and_update_cdcl_all_struct_inv inv apply auto[1]
+    using add_confl.hyps(1,2,4) add_new_clause_and_update_def 
+    cdcl_all_struct_inv_add_new_clause_and_update_cdcl_s_inv inv s_inv by auto
+  case 1 show ?case
+     by (metis add_confl.hyps(1,2,4,5) add_new_clause_and_update_def 
+       cdcl_all_struct_inv_add_new_clause_and_update_cdcl_all_struct_inv 
+       rtranclp_cdcl_all_struct_inv_inv rtranclp_cdcl_s_rtranclp_cdcl full_def inv)
+
+  case 2  show ?case
+    by (metis inv_s_T add_confl.hyps(1,2,4,5) add_new_clause_and_update_def 
+      cdcl_all_struct_inv_add_new_clause_and_update_cdcl_all_struct_inv full_def inv 
+      rtranclp_cdcl_s_cdcl_s_invariant)
+next
+  case (add_no_confl C)
+  case 1 show ?case sorry
+  case 2 show ?case sorry
+qed
 
 lemma blocked_induction_with_marked:
   assumes
